examples/Collatz_Conjecture.thy
@@ -1,20 +1,18 @@
 theory Collatz_Conjecture
-  imports "ITree_UTP.ITree_UTP"
-begin lit_vars
+  imports "ITree_UTP.ITree_VCG"
+begin
 
 zstore state = 
   n :: nat
   hist :: "nat list"
 
 procedure collatz "N :: nat" over state = 
-  "n := N \<Zcomp>
-   hist := [n] \<Zcomp>
+  "n := N ;
+   hist := [n] ;
    while n \<noteq> 1 inv True do
-     if even n then n := n div 2 else n := 3*n + 1 fi \<Zcomp>
+     if even n then n := n div 2 else n := 3*n + 1 fi ;
      hist := hist @ [n]
    od"
-
-def_consts MAX_SIL_STEPS = 200
 
 execute "collatz 2"
 execute "collatz 3"
