examples/DwarfSignal.thy
@@ -1,7 +1,7 @@
 section \<open> Dwarf Signal \<close>
 
 theory DwarfSignal
-  imports "Interaction_Trees.ITree_Simulation" "Interaction_Trees.ITree_Eval"
+  imports "ITree_Simulation.ITree_Simulation" "Interaction_Trees.ITree_Eval"
 begin                
 
 subsection \<open> State Space \<close>
