examples/List_Reversal.thy
@@ -1,23 +1,13 @@
 theory List_Reversal
-  imports "ITree_UTP.ITree_UTP"
+  imports "ITree_UTP.ITree_VCG"
 begin 
-
-term "[\<lambda> s. R i s]\<^sub>e"
-term "[\<lambda> s. R s i]\<^sub>e"
-
-lit_vars
-
-syntax
-  "_kleisli_comp" :: "logic \<Rightarrow> logic \<Rightarrow> logic" (infixr ";" 54)
-
-def_consts MAX_SIL_STEPS = 100
 
 zstore state =
   ys :: "int list"
   i :: nat
 
 procedure reverse "xs :: int list" over state =
-"ys := [] ; i := 0 ; 
+"ys := []; i := 0; 
  while i < length xs inv ys = rev (take i xs) 
  do 
     ys := xs!i # ys; 
