ROOT
@@ -14,4 +14,5 @@ session "ITree_UTP" in "UTP" = "Interaction_Trees" +
   options [timeout = 600, document = false]
   theories
     ITree_UTP
+    ITree_VCG
   
